Logic/Modal/Standard/Kripke/Ver.lean
@@ -1,10 +1,13 @@
 import Logic.Vorspiel.BinaryRelations
 import Logic.Modal.Standard.Kripke.Completeness
 
+abbrev LO.Kripke.IsolatedFrameClass : FrameClass := λ F => Isolated F
+
 namespace LO.Modal.Standard
 
 namespace Kripke
 
+open LO.Kripke
 open System
 open Kripke
 open Formula
@@ -12,12 +15,16 @@ open DeductionParameter (Normal)
 
 variable {α : Type u} [Inhabited α] [DecidableEq α]
 
-abbrev IsolatedFrameClass : FrameClass := { F | Isolated F }
+instance Ver_characterizable : 𝔽(𝐕𝐞𝐫 of α).Characteraizable (IsolatedFrameClass) := characterizable_of_valid_axiomset
+  ⟨⟨PUnit,  λ _ _ => False⟩, by tauto⟩
+  (by
+    simp;
+    intro p F hF V x y Rxy;
+    have := hF Rxy;
+    contradiction;
+  )
 
-lemma IsolatedFrameClass.nonempty : IsolatedFrameClass.Nonempty.{0} := by
-  use PointFrame
-  simp [Isolated];
-
+/-
 lemma axiomVer_defines : AxiomSet.DefinesKripkeFrameClass (α := α) 𝗩𝗲𝗿 IsolatedFrameClass := by
   simp [AxiomSet.DefinesKripkeFrameClass, Kripke.ValidOnFrame];
   intro F;
@@ -27,17 +34,20 @@ lemma axiomVer_defines : AxiomSet.DefinesKripkeFrameClass (α := α) 𝗩𝗲�
   . intro hIrrefl _ _ x y hxy;
     have := hIrrefl hxy;
     contradiction;
+-/
 
-instance : Sound (𝐕𝐞𝐫 : DeductionParameter α) IsolatedFrameClass# := sound_of_defines axiomVer_defines
+instance : Sound 𝐕𝐞𝐫 (IsolatedFrameClass#α) := inferInstance
 
-instance : System.Consistent (𝐕𝐞𝐫 : DeductionParameter α) := consistent_of_defines axiomVer_defines IsolatedFrameClass.nonempty
+instance : System.Consistent (𝐕𝐞𝐫 : DeductionParameter α) := inferInstance
 
 lemma isolated_CanonicalFrame {Ax : AxiomSet α} (h : 𝗩𝗲𝗿 ⊆ Ax) [System.Consistent 𝝂Ax] : Isolated (CanonicalFrame 𝝂Ax) := by
   intro x y rxy;
   have : (CanonicalModel 𝝂Ax) ⊧ □⊥ := iff_valid_on_canonicalModel_deducible.mpr $ Normal.maxm! (by aesop);
   exact this x _ rxy;
 
-instance : Complete (𝐕𝐞𝐫 : DeductionParameter α) IsolatedFrameClass.{u}# := instComplete_of_mem_canonicalFrame $ isolated_CanonicalFrame (by rfl)
+instance : Complete 𝐕𝐞𝐫 (IsolatedFrameClass.{u}#α) := instComplete_of_mem_canonicalFrame (IsolatedFrameClass) $ by
+  apply isolated_CanonicalFrame;
+  tauto;
 
 end Kripke
 
