Logic/Modal/Standard/Kripke/Reducible.lean
@@ -7,11 +7,12 @@ open DeductionParameter Normal
 
 namespace Kripke
 
+open LO.Kripke
 open Formula
 
 variable {α : Type*} {Ax₁ Ax₂ : AxiomSet α} (𝔽₁ 𝔽₂ : FrameClass)
-  [sound₁ : Sound 𝝂Ax₁ 𝔽₁#] [sound₂ : Sound 𝝂Ax₂ 𝔽₂#]
-  [complete₁ : Complete 𝝂Ax₁ 𝔽₁#] [complete₂ : Complete 𝝂Ax₂ 𝔽₂#]
+  [sound₁ : Sound 𝝂Ax₁ (𝔽₁#α)] [sound₂ : Sound 𝝂Ax₂ (𝔽₂#α)]
+  [complete₁ : Complete 𝝂Ax₁ (𝔽₁#α)] [complete₂ : Complete 𝝂Ax₂ (𝔽₂#α)]
 
 lemma reducible_of_subset_FrameClass (h𝔽 : 𝔽₂ ⊆ 𝔽₁) : 𝝂Ax₁ ≤ₛ 𝝂Ax₂ := by
   apply System.weakerThan_iff.mpr;
@@ -23,9 +24,7 @@ lemma reducible_of_subset_FrameClass (h𝔽 : 𝔽₂ ⊆ 𝔽₁) : 𝝂Ax₁ �
 lemma equiv_of_eq_FrameClass (h𝔽 : 𝔽₁ = 𝔽₂) : 𝝂Ax₁ =ₛ 𝝂Ax₂ := by
   apply System.Equiv.antisymm_iff.mpr;
   constructor;
-  . apply reducible_of_subset_FrameClass 𝔽₁ 𝔽₂;
-    subst_vars; rfl;
-  . apply reducible_of_subset_FrameClass 𝔽₂ 𝔽₁;
-    subst_vars; rfl;
+  . apply reducible_of_subset_FrameClass 𝔽₁ 𝔽₂; subst_vars; rfl;
+  . apply reducible_of_subset_FrameClass 𝔽₂ 𝔽₁; subst_vars; rfl;
 
 end LO.Modal.Standard.Kripke
